Fixed constant

Weidenbach_Book/Pairing_Heap/Double_Linorder.thy
@@ -310,7 +310,7 @@ definition evsids_rescore_factor :: \<open>double\<^sub>p\<close> where
 text \<open>EVSIDS needs a constant that increases our inc, in order to have the implicit decay happening\<close>
 text \<open>Here I went with \<approx> 1/0.95 as the factor\<close>
 definition evsids_decay_factor_word :: \<open>64 word\<close> where
-  \<open>evsids_decay_factor_word = 0x3FF0D79435E53BC5\<close> 
+  \<open>evsids_decay_factor_word = 0x3FF0D79435E50D79\<close> 
 
 definition evsids_decay_factor :: \<open>double\<^sub>p\<close> where
   \<open>evsids_decay_factor = const_double\<^sub>p evsids_decay_factor_word\<close>
@@ -478,13 +478,13 @@ lemma double\<^sub>p_fmul\<^sub>p_mono: \<open>(x::double\<^sub>p) \<le> y \<Lon
   by transfer (rule float\<^sub>p_fmul\<^sub>p_mono)
 
 subsubsection \<open>Constant helpers\<close>
-lemma evsids_limit_word_positive: \<open>is_positive_float (float_of_fp64 0x5F30000000000000)\<close>
+lemma evsids_limit_word_positive: \<open>is_positive_float (float_of_fp64 evsids_limit_word)\<close>
   by eval
 
-lemma evsids_limit_word_nonZero: \<open>\<not>is_zero (float_of_fp64 0x5F30000000000000)\<close>
+lemma evsids_limit_word_nonZero: \<open>\<not>is_zero (float_of_fp64 evsids_limit_word)\<close>
   by eval
 
-lemma evsids_limit_word_nonInf: \<open>\<not>is_infinity (float_of_fp64 0x5F30000000000000)\<close>
+lemma evsids_limit_word_nonInf: \<open>\<not>is_infinity (float_of_fp64 evsids_limit_word)\<close>
   by eval
 
 lemma evsids_limit_nonZero: \<open>\<not>is_zero\<^sub>p evsids_limit\<close>
@@ -495,16 +495,16 @@ lemma evsids_limit_nonInf: \<open>\<not>is_infinity\<^sub>p evsids_limit\<close>
 
 lemma mop_dpconst_evsids_limit[simp]:
   \<open>mop_dpconst evsids_limit_word = RETURN evsids_limit\<close>
-  unfolding mop_dpconst_def evsids_limit_def evsids_limit_word_def
+  unfolding mop_dpconst_def evsids_limit_def
   by (simp add: evsids_limit_word_positive)
 
-lemma evsids_rescore_factor_word_positive: \<open>is_positive_float (float_of_fp64 0x20B0000000000000)\<close>
+lemma evsids_rescore_factor_word_positive: \<open>is_positive_float (float_of_fp64 evsids_rescore_factor_word)\<close>
   by eval
 
-lemma evsids_rescore_factor_word_nonZero: \<open>\<not>is_zero (float_of_fp64 0x20B0000000000000)\<close>
+lemma evsids_rescore_factor_word_nonZero: \<open>\<not>is_zero (float_of_fp64 evsids_rescore_factor_word)\<close>
   by eval
 
-lemma evsids_rescore_factor_word_nonInf: \<open>\<not>is_infinity (float_of_fp64 0x20B0000000000000)\<close>
+lemma evsids_rescore_factor_word_nonInf: \<open>\<not>is_infinity (float_of_fp64 evsids_rescore_factor_word)\<close>
   by eval
 
 lemma evsids_rescore_factor_nonZero: \<open>\<not>is_zero\<^sub>p evsids_rescore_factor\<close>
@@ -515,16 +515,16 @@ lemma evsids_rescore_factor_nonInf: \<open>\<not>is_infinity\<^sub>p evsids_resc
 
 lemma mop_dpconst_evsids_rescore_factor[simp]:
   \<open>mop_dpconst evsids_rescore_factor_word = RETURN evsids_rescore_factor\<close>
-  unfolding mop_dpconst_def evsids_rescore_factor_def evsids_rescore_factor_word_def
+  unfolding mop_dpconst_def evsids_rescore_factor_def
   by (simp add: evsids_rescore_factor_word_positive)
 
-lemma evsids_decay_factor_word_positive: \<open>is_positive_float (float_of_fp64 0x3FF0D79435E53BC5)\<close>
+lemma evsids_decay_factor_word_positive: \<open>is_positive_float (float_of_fp64 evsids_decay_factor_word)\<close>
   by eval
 
-lemma evsids_decay_factor_word_nonZero: \<open>\<not>is_zero (float_of_fp64 0x3FF0D79435E53BC5)\<close>
+lemma evsids_decay_factor_word_nonZero: \<open>\<not>is_zero (float_of_fp64 evsids_decay_factor_word)\<close>
   by eval
 
-lemma evsids_decay_factor_word_nonInf: \<open>\<not>is_infinity (float_of_fp64 0x3FF0D79435E53BC5)\<close>
+lemma evsids_decay_factor_word_nonInf: \<open>\<not>is_infinity (float_of_fp64 evsids_decay_factor_word)\<close>
   by eval
 
 lemma evsids_decay_factor_nonZero: \<open>\<not>is_zero\<^sub>p evsids_decay_factor\<close>
@@ -535,7 +535,7 @@ lemma evsids_decay_factor_nonInf: \<open>\<not>is_infinity\<^sub>p evsids_decay_
 
 lemma mop_dpconst_evsids_decay_factor[simp]:
   \<open>mop_dpconst evsids_decay_factor_word = RETURN evsids_decay_factor\<close>
-  unfolding mop_dpconst_def evsids_decay_factor_def evsids_decay_factor_word_def
+  unfolding mop_dpconst_def evsids_decay_factor_def
   by (simp add: evsids_decay_factor_word_positive)
 
 subsection \<open>Sepref constants\<close>
